extraction/extraction.v
@@ -4,15 +4,29 @@ Require Import FreeSpec.Program.
 Require Import FreeSpec.Oracle.Oracle.
 
 Require Import FreeSpec.Examples.Map.
+Require Import FreeSpec.Specs.Memory.
 
+(** * Haskell Extraction Plugin
+ *)
 Add LoadPath "./libs/haskell-extraction/ocaml/".
 
 Require Import HaskellExtraction.HaskellExtraction.
 
-Extraction Language Haskell.
-
 Hextraction , Map.IMap.
 
+(** * Ocaml Regular Extraction
+
+ *)
+
+Extraction Language Haskell.
+
+Require Import ExtrHaskellBasic.
+Require Import ExtrHaskellNatInt.
+
+Extract Inlined Constant Datatypes.fst => "fst".
+Extract Inlined Constant Datatypes.snd => "snd".
+
 Extraction "FreeSpec"
-           Program.Program Program.runProgram'
-           Map.IMap test_interpreter.
+           Program.runProgram' Memory.mem
+           Control.Identity.Identity Control.Identity.identity_Monad
+           Memory.append Map.IMap test_interpreter.
